cfi: working on qa refinement - broken state

cfi/qa.v
@@ -33,6 +33,14 @@ Class sym_cfi_params := {
 
 Context {scp : sym_cfi_params}.
 
+Class params_spec (sp : sym_cfi_params) := {
+
+  mem_axioms : PartMaps.axioms get_mem upd_mem;
+  
+  reg_axioms : PartMaps.axioms get_reg upd_reg
+
+}.
+
 Variable valid_jmp : word t -> word t -> bool.
 
 Program Instance sym_cfi : (Symbolic.symbolic_params t) := {
@@ -60,12 +68,12 @@ Local Notation "x .+1" := (add_word x (Z_to_word 1)) (at level 60).
 
 Open Scope word_scope.
 
-Definition csucc (st : Abstract.state t) (st' : Abstract.state t) : bool :=
-  let pc_t' := common.tag (Abstract.pc st') in
-  let pc_t := common.tag (Abstract.pc st) in
-  let pc_s := common.val (Abstract.pc st) in
-  let pc_s' := common.val (Abstract.pc st') in
-  match (get_mem (Abstract.mem st) pc_s) with
+Definition ssucc (st : Symbolic.state t) (st' : Symbolic.state t) : bool :=
+  let pc_t' := common.tag (Symbolic.pc st') in
+  let pc_t := common.tag (Symbolic.pc st) in
+  let pc_s := common.val (Symbolic.pc st) in
+  let pc_s' := common.val (Symbolic.pc st') in
+  match (get_mem (Symbolic.mem st) pc_s) with
     | Some i =>
       match decode_instr (common.val i) with
         | Some (Jump r) => valid_jmp pc_s pc_s'
@@ -90,7 +98,7 @@ Program Instance symbolic_cfi_machine : cfi_machine t := {|
 
   get_pc s := common.val (Symbolic.pc s);
   
-  succ := csucc      
+  succ := ssucc      
  |}.
 Next Obligation.
 Admitted.
